SL/ListReversal.thy
@@ -9,10 +9,19 @@ record rev_list =
   k :: nat
 
 
-find_consts name: j_update
+lemma "ht (list_seg (Cons x xs) i k)
+    (
+      lookup j_update (\<lambda>s. (i s) + 1);
+      dispose i;
+      dispose (\<lambda>s. i s + 1);
+      assign i_update j
+    )
+    (list_seg xs i k)"
+apply hoare 
+sorry
 
 lemma "spec (llist xs i) (llist (rev xs) j) \<le> (
-      assign j_update #0;
+      assign j_update $0;
       while ({(s, h). i s \<noteq> 0}) 
         (
           lookup k_update (\<lambda>s. i s + 1);
@@ -23,51 +32,51 @@ lemma "spec (llist xs i) (llist (rev xs) j) \<le> (
       )"
 proof -
   have "spec (llist xs i) (llist (rev xs) j) \<le>
-      assign j_update #0; 
+      assign j_update $0; 
       (spec (EXS A B. llist A i * llist B j * <{s. rev xs = (rev A) @ B}>) (llist (rev xs) j))"
       by morgan (sep_auto, auto)
   also have "... \<le> 
-      assign j_update #0; 
+      assign j_update $0; 
       while ({(s, h). i s \<noteq> 0})  (
         (spec (EXS A B. llist A i * llist B j * <{s. rev xs = (rev A) @ B}> * <{s. i s \<noteq> 0}>)
               (EXS A B. llist A i * llist B j * <{s. rev xs = (rev A) @ B}>))
       )"
       by morgan sep_auto+
   also have "... \<le> 
-      assign j_update #0; 
+      assign j_update $0; 
       while ({(s, h). i s \<noteq> 0})  (
-        (spec (EXS A B a k. (i \<mapsto> #a, #k) * llist A #k * llist B j * <{s. rev xs = (rev (Cons a A)) @ B}> * <{s. i s \<noteq> 0}>)
+        (spec (EXS A B a k. (i \<mapsto> $a, $k) * llist A $k * llist B j * <{s. rev xs = (rev (Cons a A)) @ B}> * <{s. i s \<noteq> 0}>)
               (EXS A B. llist A i * llist B j * <{s. rev xs = (rev A) @ B}>))
       )"
       by morgan (sep_safe, sep_auto)
   also have "... \<le> 
-      assign j_update #0; 
+      assign j_update $0; 
       while ({(s, h). i s \<noteq> 0})  (
         lookup k_update (\<lambda>s. i s + 1);
-        (spec (EXS A B a. (i \<mapsto> #a, k) * llist A k * llist B j * <{s. rev xs = (rev (Cons a A)) @ B}> * <{s. i s \<noteq> 0}>)
+        (spec (EXS A B a. (i \<mapsto> $a, k) * llist A k * llist B j * <{s. rev xs = (rev (Cons a A)) @ B}> * <{s. i s \<noteq> 0}>)
               (EXS A B. llist A i * llist B j * <{s. rev xs = (rev A) @ B}>))
       )"
       by morgan sep_auto+
   also have "... \<le> 
-      assign j_update #0; 
+      assign j_update $0; 
       while ({(s, h). i s \<noteq> 0})  (
         lookup k_update (\<lambda>s. i s + 1);
         mutation (\<lambda>s. i s + 1) j;
-        (spec (EXS A B a. (i \<mapsto> #a, j) * llist A k * llist B j * <{s. rev xs = (rev (Cons a A)) @ B}> * <{s. i s \<noteq> 0}>)
+        (spec (EXS A B a. (i \<mapsto> $a, j) * llist A k * llist B j * <{s. rev xs = (rev (Cons a A)) @ B}> * <{s. i s \<noteq> 0}>)
               (EXS A B. llist A i * llist B j * <{s. rev xs = (rev A) @ B}>))
       )"
     by morgan
   also have "... \<le> 
-      assign j_update #0; 
+      assign j_update $0; 
       while ({(s, h). i s \<noteq> 0})  (
         lookup k_update (\<lambda>s. i s + 1);
         mutation (\<lambda>s. i s + 1) j;
-        (spec (EXS A B a. llist A k * (i \<mapsto> #a, j) * llist B j * <{s. rev xs = (rev (Cons a A)) @ B}> * <{s. i s \<noteq> 0}>)
+        (spec (EXS A B a. llist A k * (i \<mapsto> $a, j) * llist B j * <{s. rev xs = (rev (Cons a A)) @ B}> * <{s. i s \<noteq> 0}>)
               (EXS A B. llist A i * llist B j * <{s. rev xs = (rev A) @ B}>))
       )"
     by morgan sep_auto
     also have "... \<le> 
-      assign j_update #0; 
+      assign j_update $0; 
       while ({(s, h). i s \<noteq> 0})  (
         lookup k_update (\<lambda>s. i s + 1);
         mutation (\<lambda>s. i s + 1) j;
@@ -76,7 +85,7 @@ proof -
       )"
       by morgan sep_auto
     also have "... \<le> 
-      assign j_update #0; 
+      assign j_update $0; 
       while ({(s, h). i s \<noteq> 0})  (
         lookup k_update (\<lambda>s. i s + 1);
         mutation (\<lambda>s. i s + 1) j;
@@ -85,7 +94,7 @@ proof -
       )"
       by morgan sep_auto+
     also have "... \<le> 
-      assign j_update #0; 
+      assign j_update $0; 
       while ({(s, h). i s \<noteq> 0})  (
         lookup k_update (\<lambda>s. i s + 1);
         mutation (\<lambda>s. i s + 1) j;
@@ -95,7 +104,7 @@ proof -
       )"
       by morgan sep_auto
     also have "... \<le> 
-      assign j_update #0; 
+      assign j_update $0; 
       while ({(s, h). i s \<noteq> 0})  (
         lookup k_update (\<lambda>s. i s + 1);
         mutation (\<lambda>s. i s + 1) j;
@@ -107,25 +116,30 @@ proof -
 qed
 
 
+lemma reynolds6_var: "P \<le> (e \<mapsto> e' x) * true \<Longrightarrow> P \<le> Q \<Longrightarrow> P \<le> (EXS x. (e \<mapsto> e' x) * ((e \<mapsto> e' x) -* Q)) "
+  sorry
+
+lemma lookup_ref452 [sl]:"ht (EXS x. (v \<mapsto> (\<lambda>_. a), (\<lambda>_. x)) * R (\<lambda>_. x)) (lookup k_upd (\<lambda>s. v s + 1)) ((v \<mapsto> b, kei) * R kei)"
+sorry
+
+lemma mutation_ref452 [sl]: "ht (v \<mapsto> a, b) (mutation (\<lambda>s. v s + 1) e) (v \<mapsto> a, e)"
+  sorry
+
 lemma "ht (llist xs i)(
-      assign j_update #0;
+      assign j_update $0;
       awhile (EXS as bs. (llist as i * llist bs j) * (<{s. rev xs = rev as @ bs}>))
         ({(s, h). i s \<noteq> 0}) 
         (
-          lookup k_update (\<lambda>s. i s + 1);
-          mutation (\<lambda>s. i s + 1) j;
+          apre (EXS A B a k. (i \<mapsto> $a, $k) * llist A $k * llist B j * <{s. rev xs = (rev (Cons a A)) @ B}> * <{s. i s \<noteq> 0}>)
+          (lookup k_update (\<lambda>s. i s + 1));
+          apost 
+          (mutation (\<lambda>s. i s + 1) j)
+          ((EXS A B a. (i \<mapsto> $a, j) * llist A k * llist B j * <{s. rev xs = (rev (Cons a A)) @ B}> * <{s. i s \<noteq> 0}>));
           assign j_update i;
           assign i_update k
         )
       )(llist (rev xs) j)"
-apply hoare
-apply sep_auto
-defer
-apply sep_auto
-apply sep_auto
-defer
-defer
-apply sep_auto
+by (hoare; sep_safe) sep_auto+
 
 
 end
